theories/Logic/Kripke.v
@@ -3,90 +3,14 @@ From Coq Require Import
   Program.Basics
   Classes.Morphisms.
 
-From ExtLib Require Import Structures.Monad.
+From CTree Require Export
+  Logic.World.
+
 From CTree Require Import
   Utils.Utils
-  Events.Core
-  Events.WriterE.
+  Events.Core.
 
 Generalizable All Variables.
-
-Variant World (E:Type@{eff}) `{Encode E} :=
-  | Pure
-  | Obs (e : E) (v : encode e)
-  | Done {X} (x: X)
-  | Finish {X} (e: E) (v: encode e) (x: X).    
-Global Hint Constructors World: ctl.
-
-Arguments Pure {E} {_}.
-Arguments Obs {E} {_} e v.
-Arguments Done {E} {_} {X} x.
-Arguments Finish {E} {_} {X} e v x.
-
-Variant not_pure `{Encode E}: World E -> Prop :=
-  | NotPureObs: forall (e: E) (v: encode e),
-      not_pure (Obs e v)
-  | NotPureFinish {X}: forall (e: E) (v: encode e) (x: X),
-      not_pure (Finish e v x).
-Global Hint Constructors not_pure: ctl.
-
-Variant is_pure `{Encode E}: World E -> Prop :=
-  | IsPurePure:
-      is_pure Pure
-  | IsPureDone {X}: forall (x: X),
-      is_pure (Done x).
-Global Hint Constructors is_pure: ctl.
-
-Variant vis_with `{Encode E} (R: forall e, encode e -> Prop) : World E -> Prop :=
-  | VisWithVis: forall (e: E) (v: encode e),
-      R e v -> vis_with R (Obs e v).
-Global Hint Constructors vis_with: ctl.
-
-Variant done_with `{Encode E} {X} (R: X -> World E -> Prop): World E -> Prop :=
-  | DoneWithDone: forall (x: X),
-      R x Pure -> done_with R (Done x)
-  | DoneWithFinish: forall (e: E) (v: encode e) (x: X),
-      R x (Obs e v) -> done_with R (Finish e v x).
-Global Hint Constructors done_with: ctl.
-
-Definition done_eq `{Encode E} {X} (x: X): World E -> Prop :=
-  @done_with E H X (fun x' w' => x = x').
-
-Definition finish_with `{Encode E} {X} (R: X -> forall (e:E), encode e -> Prop) : X -> World E -> Prop :=
-  fun x w => exists (e: E) (v: encode e), w = Obs e v /\ R x e v.
-Global Hint Unfold done_eq finish_with: ctl.
-
-Variant not_done `{Encode E}: World E -> Prop :=
-  | NotDonePure: not_done Pure
-  | NotDoneObs: forall (e: E) (v: encode e),
-      not_done (Obs e v).
-Global Hint Constructors not_done: ctl.
-
-Variant is_done `{Encode E} X: World E -> Prop :=
-  | DoneDone: forall (x: X), is_done X (Done x)
-  | DoneFinish: forall (e: E) (v: encode e) (x: X),
-      is_done X (Finish e v x).
-Global Hint Constructors is_done: ctl.
-
-Definition not_done_dec `{Encode E}: forall (w: World E),
-    {not_done w} + {exists X, is_done X w}.
-Proof.
-  dependent destruction w; intros.
-  - left; econstructor.
-  - left; econstructor.
-  - right; eexists; econstructor. 
-  - right; eexists; econstructor.
-Qed.
-
-Definition not_pure_dec `{Encode E}: forall (w: World E),
-    {not_pure w} + {is_pure w}.
-Proof.
-  dependent destruction w; intros.
-  - right; econstructor. 
-  - left; econstructor.
-  - right; econstructor. 
-  - left; econstructor.
-Qed.
 
 (*| Polymorphic Kripke model over family M |*)
 Class Kripke (M: forall E, Encode E -> Type -> Type) (E: Type) `{HE: Encode E} := {
