theories/CTree/Events/Writer.v
@@ -1,23 +1,14 @@
-(*| Useful instructions: State |*)
+(*| Useful instructions: Instrumentation |*)
+
+From Coq Require Import
+  Relations.
+
 From CTree Require Import
   Classes
+  Logic.World
   CTree.Core.
 
 From CTree Require Export
   Events.WriterE.
 
-From ExtLib Require Import
-  Monoid
-  Monads
-  PPair
-  Structures.MonadWriter
-  Data.Monads.WriterMonad.
-
-Import MonadNotation.
-Local Open Scope monad_scope.
-
 Definition log {S}: S -> ctree (writerE S) unit := fun s => Ctree.trigger (Log s).
-
-#[global] Instance MonadBr_writerT {M Σ} {SM: Monoid Σ} {MM: Monad M} {AM: MonadBr M}
-  : MonadBr (writerT SM M) :=
-  fun n => @mkWriterT Σ SM M (fin (S n)) (f <- mbr n;; ret (ppair f (monoid_unit SM))).
